code/experimental/rsapss/Hacl.Spec.Bignum.fsti
@@ -24,6 +24,11 @@ val bn_sub: #aLen:size_nat -> #bLen:size_nat{bLen <= aLen} -> a:lbignum aLen -> 
 val bn_sub_lemma: #aLen:size_nat -> #bLen:size_nat{bLen <= aLen} -> a:lbignum aLen -> b:lbignum bLen ->
   Lemma (let (c_out, res) = bn_sub a b in bn_v res - v c_out * pow2 (64 * aLen) == bn_v a - bn_v b)
 
+val bn_add_mod_n: #len:size_nat -> n:lbignum len -> a:lbignum len -> b:lbignum len -> lbignum len
+
+val bn_add_mod_n_lemma: #len:size_nat -> n:lbignum len -> a:lbignum len -> b:lbignum len -> Lemma
+  (requires bn_v a < bn_v n /\ bn_v b < bn_v n)
+  (ensures  bn_v (bn_add_mod_n n a b) == (bn_v a + bn_v b) % bn_v n)
 
 val bn_mul: #aLen:size_nat -> #bLen:size_nat{aLen + bLen <= max_size_t} -> a:lbignum aLen -> b:lbignum bLen -> lbignum (aLen + bLen)
 
